generic/Zeta.Generic.Global.fsti
@@ -1,0 +1,33 @@
+module Zeta.Generic.Global
+
+open FStar.Seq
+open Zeta.SeqAux
+open Zeta.Interleave
+open Zeta.Time
+open Zeta.GenericVerifier
+open Zeta.Generic.Thread
+
+module S = FStar.Seq
+module SA = Zeta.SeqAux
+module T = Zeta.Generic.Thread
+module I = Zeta.Interleave
+
+(* a global log is a collection of thread-level verifier logs *)
+let vlog (vspec: verifier_spec) = seq (verifier_log vspec)
+
+let thread_log #vspec (gl: vlog vspec) (tid: SA.seq_index gl): T.vlog _ =
+  (tid, S.index gl tid)
+
+let index #vspec (gl: vlog vspec) (i: sseq_index gl) =
+  I.indexss gl i
+
+(* a global log is verifiable if every thread-level log is verifiable *)
+let verifiable #vspec (gl: vlog vspec) =
+  forall (tid: SA.seq_index gl). {:pattern T.verifiable (thread_log gl tid)} T.verifiable (thread_log gl tid)
+
+let verifiable_log vspec = gl:vlog vspec {verifiable gl}
+
+let clock #vspec (gl: verifiable_log vspec) (i: sseq_index gl) =
+  let tid, i' = i in
+  let tl = thread_log gl tid in
+  T.clock tl i'
