generic/Zeta.Generic.TSLog.fsti
@@ -1,0 +1,45 @@
+module Zeta.Generic.TSLog
+
+open Zeta.SeqAux
+open Zeta.Interleave
+open Zeta.Time
+open Zeta.GenericVerifier
+open Zeta.Generic.Thread
+open Zeta.Generic.Global
+
+module V = Zeta.GenericVerifier
+module T = Zeta.Generic.Thread
+module G = Zeta.Generic.Global
+module I = Zeta.Interleave
+
+let ilog (vspec: verifier_spec) = interleaving (verifier_log_entry vspec)
+
+(* valid thread ids of an interleaving *)
+let thread_id #vspec (il: ilog vspec) = Zeta.Thread.thread_id
+
+(* to sequence of individual thread-level logs *)
+let to_gvlog #vspec (il: ilog vspec): G.vlog _
+  = I.s_seq il
+
+(* an interleaving is verifiable is the source logs are verifiable *)
+let verifiable #vspec (il: ilog vspec) =
+  G.verifiable (to_gvlog il)
+
+let seq_index #vspec (il: ilog vspec) = I.seq_index il
+
+let prefix #vspec (il: ilog vspec) = I.prefix il
+
+let clock #vspec (il: ilog vspec {verifiable il}) (i: seq_index il) =
+  let j = i2s_map il i in
+  G.clock (to_gvlog il) j
+
+let clock_sorted (#vspec:_) (il: ilog vspec {verifiable il}) =
+  forall (i j: I.seq_index il). i <= j ==> clock il i `ts_leq` clock il j
+
+let its_log vspec = il:ilog vspec{verifiable il /\ clock_sorted il}
+
+val lemma_prefix_verifiable (#vspec:_) (itsl: its_log vspec) (i:nat{i <= I.length itsl}):
+  Lemma (ensures (verifiable (I.prefix itsl i) /\ clock_sorted (I.prefix itsl i)))
+        [SMTPat (I.prefix itsl i)]
+
+val create (#vspec:_) (gl: verifiable_log vspec): (itsl:its_log vspec{to_gvlog itsl == gl})
