generic/Zeta.Generic.Thread.fst
@@ -1,0 +1,101 @@
+module Zeta.Generic.Thread
+
+(* if a thread log is verifiable, its prefix is verifiable *)
+let rec verifiable_implies_prefix_verifiable (#vspec:verifier_spec)
+  (tl:verifiable_log vspec) (i:nat{i <= length tl}):
+  Lemma (ensures (verifiable (prefix tl i)))
+        (decreases (length tl))
+  = let n = length tl in
+    if n = i then ()
+    else verifiable_implies_prefix_verifiable (prefix tl (n-1)) i
+
+(* the state after processing i'th entry is obtained by applying the verify
+ * step to the state before processing the i'th entry *)
+let lemma_state_transition (#vspec:verifier_spec) (tl: verifiable_log vspec) (i: seq_index tl):
+  Lemma (ensures (state_at tl (i + 1) ==
+                  verify_step (index tl i) (state_at tl i)))
+  = ()
+
+let rec lemma_clock_monotonic (#vspec:verifier_spec)
+  (tl: verifiable_log vspec) (i:nat) (j: seq_index tl {j >= i}):
+  Lemma (ensures (clock tl i `ts_leq` clock tl j))
+  (decreases (i + j + length tl))
+  = let n = length tl - 1 in
+    let tl' = prefix tl n in
+    if j < n
+    then lemma_clock_monotonic tl' i j
+    else if i = j then ()
+    else lemma_clock_monotonic tl i (j-1)
+
+(* the thread id in the state is always the one specified in the parameter *)
+let rec lemma_thread_id_state (#vspec:verifier_spec) (tl: verifiable_log vspec):
+  Lemma (ensures (let tid, _ = tl in
+                  vspec.tid (verify tl) = tid))
+        (decreases (length tl))
+  = let n = length tl in
+    if n = 0 then ()
+    else lemma_thread_id_state (prefix tl (n-1))
+
+let add_epoch_filter #vspec (ep: epoch) (tl: verifiable_log vspec): ((seq_index tl) -> bool)
+  = let _,l = tl in
+    let f = fun (i: SA.seq_index l) ->
+            let e = S.index l i in
+            is_blum_add e &&
+            (let be = blum_add_elem e in
+            epoch_of be = ep) in
+    f
+
+let to_blum_add_elem #vspec (ep: epoch) (tl: verifiable_log vspec):
+  (i:seq_index tl{add_epoch_filter ep tl i} -> ms_hashfn_dom vspec.app)
+  = let _,l = tl in
+    let f = add_epoch_filter ep tl in
+    let m = fun (i: SA.seq_index l { f i }) ->
+            let e = S.index l i in
+            blum_add_elem e in
+    m
+
+let blum_add_seq (#vspec: verifier_spec) (ep: epoch) (tl: verifiable_log vspec):
+  S.seq (ms_hashfn_dom vspec.app)
+  = let _,l = tl in
+    let f = add_epoch_filter ep tl in
+    let m = to_blum_add_elem ep tl in
+    SA.indexed_filter_map l f m
+
+let add_seq_map
+  (#vspec: verifier_spec)
+  (tl: verifiable_log vspec)
+  (i: seq_index tl {is_blum_add (index tl i)}):
+  (let be = blum_add_elem (index tl i) in
+   let ep = epoch_of be in
+   let add_seq = blum_add_seq ep tl in
+   j: SA.seq_index add_seq{S.index add_seq j = be})
+  = let be = blum_add_elem (index tl i) in
+    let ep = epoch_of be in
+    let _,l = tl in
+    let f = add_epoch_filter ep tl in
+    let m = to_blum_add_elem ep tl in
+    SA.indexed_filter_map_map l f m i
+
+let add_seq_inv_map
+  (#vspec: verifier_spec)
+  (ep: epoch)
+  (tl: verifiable_log vspec)
+  (j: SA.seq_index (blum_add_seq ep tl)):
+  (i: seq_index tl {is_blum_add (index tl i) /\
+                    blum_add_elem (index tl i) = S.index (blum_add_seq ep tl) j /\
+                    epoch_of (blum_add_elem (index tl i)) = ep /\
+                    add_seq_map tl i = j})
+ = let _,l = tl in
+   let f = add_epoch_filter ep tl in
+   let m = to_blum_add_elem ep tl in
+   SA.indexed_filter_map_invmap l f m j
+
+
+let lemma_add_seq_inv
+  (#vspec:_)
+  (tl: verifiable_log vspec)
+  (i: seq_index tl{is_blum_add (index tl i)}):
+  Lemma (ensures (let be = blum_add_elem (index tl i) in
+                  let ep = epoch_of be in
+                  add_seq_inv_map ep tl (add_seq_map tl i) = i))
+  = ()
